TwoColouringEx.thy
@@ -11,61 +11,105 @@ declare [[coercion cast_ruleschema_rule]]
 
 
 definition init :: ruleschema where
-"init = \<lparr>rule_ty = [''a'' \<mapsto> Lty],
-         rule_lhs = \<lparr>nodes = [1 \<mapsto> \<lparr>node_mark = RuleMarkNode_None, node_label= Var ''a'' # [], node_rooted=False\<rparr>]
-                   ,edges = Map.empty\<rparr>,
-         rule_rhs = \<lparr>nodes = [1 \<mapsto> \<lparr>node_mark = RuleMarkNode_Red, node_label= Var ''a'' # [] , node_rooted=False\<rparr>]
-               ,edges = Map.empty\<rparr>,
+"init = \<lparr>rule_ty = Mapping [(0,Lty)],
+         rule_lhs = \<lparr>nodes = Mapping [(1, \<lparr>node_mark = RuleMarkNode_None, node_label= Var 0 # [], node_rooted=False\<rparr>)]
+                   ,edges = Mapping.empty\<rparr>,
+         rule_rhs = \<lparr>nodes = Mapping [(1, \<lparr>node_mark = RuleMarkNode_Red, node_label= Var 0 # [] , node_rooted=False\<rparr>)]
+               ,edges = Mapping.empty\<rparr>,
          rule_interf = {1}\<rparr>"
 
 definition unmark :: rule where
-"unmark = (\<lparr>rule_ty = [''a'' \<mapsto> Lty],
-           rule_lhs = \<lparr>nodes = [1 \<mapsto> \<lparr>node_mark = RuleMarkNode_Any, node_label= Var ''a'' # [] , node_rooted=False\<rparr>]
-                 ,edges = Map.empty\<rparr>,
-           rule_rhs = \<lparr>nodes = [1 \<mapsto> \<lparr>node_mark = RuleMarkNode_None, node_label= Var ''a'' # [], node_rooted=False\<rparr>]
-                 ,edges = Map.empty\<rparr>,
+"unmark = (\<lparr>rule_ty = Mapping [(0, Lty)],
+           rule_lhs = \<lparr>nodes = Mapping [(1, \<lparr>node_mark = RuleMarkNode_Any, node_label= Var 0 # [] , node_rooted=False\<rparr>)]
+                 ,edges = Mapping.empty\<rparr>,
+           rule_rhs = \<lparr>nodes = Mapping[(1, \<lparr>node_mark = RuleMarkNode_None, node_label= Var 0 # [], node_rooted=False\<rparr>)]
+                 ,edges = Mapping.empty\<rparr>,
            rule_interf = {1}\<rparr>, cond.T)"
 
-definition col_blue :: ruleschema where
-"col_blue = \<lparr>rule_ty = [''a'' \<mapsto> Lty, ''b'' \<mapsto> Lty, ''c'' \<mapsto> Lty]
-            ,rule_lhs = \<lparr>nodes = [1 \<mapsto> \<lparr>node_mark = RuleMarkNode_Red , node_label = [Var ''a''], node_rooted = False\<rparr>
-                                 ,1 \<mapsto> \<lparr>node_mark = RuleMarkNode_None, node_label = [Var ''b''], node_rooted = False\<rparr>]
-                        ,edges = [1 \<mapsto> \<lparr>edge_src = 1, edge_trg = 2, edge_mark = RuleMarkEdge_None, edge_label = [Var ''c'']\<rparr>]\<rparr>
-            ,rule_rhs = \<lparr>nodes = [1 \<mapsto> \<lparr>node_mark = RuleMarkNode_Red , node_label = [Var ''a''], node_rooted = False\<rparr>
-                                 ,1 \<mapsto> \<lparr>node_mark = RuleMarkNode_Blue, node_label = [Var ''b''], node_rooted = False\<rparr>]
-                        ,edges = [1 \<mapsto> \<lparr>edge_src = 1, edge_trg = 2, edge_mark = RuleMarkEdge_None, edge_label = [Var ''c'']\<rparr>]\<rparr>
+definition col_blue_1 :: ruleschema where
+"col_blue_1 = \<lparr>rule_ty = Mapping [(0, Lty), (1, Lty), (2, Lty)]
+            ,rule_lhs = \<lparr>nodes = Mapping
+                                 [(1, \<lparr>node_mark = RuleMarkNode_Red , node_label = [Var 0], node_rooted = False\<rparr>)
+                                 ,(2, \<lparr>node_mark = RuleMarkNode_None, node_label = [Var 1], node_rooted = False\<rparr>)]
+                        ,edges = Mapping [(1, \<lparr>edge_src = 1, edge_trg = 2, edge_mark = RuleMarkEdge_None, edge_label = [Var 2]\<rparr>)]\<rparr>
+            ,rule_rhs = \<lparr>nodes = Mapping
+                                 [(1, \<lparr>node_mark = RuleMarkNode_Red , node_label = [Var 0], node_rooted = False\<rparr>)
+                                 ,(2, \<lparr>node_mark = RuleMarkNode_Blue, node_label = [Var 1], node_rooted = False\<rparr>)]
+                        ,edges = Mapping [(1, \<lparr>edge_src = 1, edge_trg = 2, edge_mark = RuleMarkEdge_None, edge_label = [Var 2]\<rparr>)]\<rparr>
+            ,rule_interf = {1,2}\<rparr>"
+
+definition col_blue_2 :: ruleschema where
+"col_blue_2 = \<lparr>rule_ty = Mapping [(0, Lty), (1, Lty), (2, Lty)]
+            ,rule_lhs = \<lparr>nodes = Mapping
+                                 [(1, \<lparr>node_mark = RuleMarkNode_Red , node_label = [Var 0], node_rooted = False\<rparr>)
+                                 ,(2, \<lparr>node_mark = RuleMarkNode_None, node_label = [Var 1], node_rooted = False\<rparr>)]
+                        ,edges = Mapping [(1, \<lparr>edge_src = 2, edge_trg = 1, edge_mark = RuleMarkEdge_None, edge_label = [Var 2]\<rparr>)]\<rparr>
+            ,rule_rhs = \<lparr>nodes = Mapping
+                                 [(1, \<lparr>node_mark = RuleMarkNode_Red , node_label = [Var 0], node_rooted = False\<rparr>)
+                                 ,(2, \<lparr>node_mark = RuleMarkNode_Blue, node_label = [Var 1], node_rooted = False\<rparr>)]
+                        ,edges = Mapping [(1, \<lparr>edge_src = 2, edge_trg = 1, edge_mark = RuleMarkEdge_None, edge_label = [Var 2]\<rparr>)]\<rparr>
             ,rule_interf = {1,2}\<rparr>"
              
-definition col_red :: ruleschema where
-"col_red = \<lparr>rule_ty = [''a'' \<mapsto> Lty, ''b'' \<mapsto> Lty, ''c'' \<mapsto> Lty]
-           ,rule_lhs = \<lparr>nodes = [1 \<mapsto> \<lparr>node_mark = RuleMarkNode_Blue , node_label = [Var ''a''], node_rooted = False\<rparr>
-                                ,1 \<mapsto> \<lparr>node_mark = RuleMarkNode_None, node_label = [Var ''b''], node_rooted = False\<rparr>]
-                       ,edges = [1 \<mapsto> \<lparr>edge_src = 1, edge_trg = 2, edge_mark = RuleMarkEdge_None, edge_label = [Var ''c'']\<rparr>]\<rparr>
-           ,rule_rhs = \<lparr>nodes = [1 \<mapsto> \<lparr>node_mark = RuleMarkNode_Blue , node_label = [Var ''a''], node_rooted = False\<rparr>
-                                ,1 \<mapsto> \<lparr>node_mark = RuleMarkNode_Red, node_label = [Var ''b''], node_rooted = False\<rparr>]
-                       ,edges = [1 \<mapsto> \<lparr>edge_src = 1, edge_trg = 2, edge_mark = RuleMarkEdge_None, edge_label = [Var ''c'']\<rparr>]\<rparr>
+definition col_red_1 :: ruleschema where
+"col_red_1 = \<lparr>rule_ty = Mapping [(0, Lty), (1, Lty), (2, Lty)]
+           ,rule_lhs = \<lparr>nodes = Mapping
+                                [(1, \<lparr>node_mark = RuleMarkNode_Blue , node_label = [Var 0], node_rooted = False\<rparr>)
+                                ,(2, \<lparr>node_mark = RuleMarkNode_None, node_label = [Var 1], node_rooted = False\<rparr>)]
+                       ,edges = Mapping [(1, \<lparr>edge_src = 1, edge_trg = 2, edge_mark = RuleMarkEdge_None, edge_label = [Var 2]\<rparr>)]\<rparr>
+           ,rule_rhs = \<lparr>nodes = Mapping 
+                                [(1, \<lparr>node_mark = RuleMarkNode_Blue , node_label = [Var 0], node_rooted = False\<rparr>)
+                                ,(2, \<lparr>node_mark = RuleMarkNode_Red, node_label = [Var 1], node_rooted = False\<rparr>)]
+                       ,edges = Mapping [(1, \<lparr>edge_src = 1, edge_trg = 2, edge_mark = RuleMarkEdge_None, edge_label = [Var 2]\<rparr>)]\<rparr>
+           ,rule_interf = {1,2}\<rparr>"
+
+             
+definition col_red_2 :: ruleschema where
+"col_red_2 = \<lparr>rule_ty = Mapping [(0, Lty), (1, Lty), (2, Lty)]
+           ,rule_lhs = \<lparr>nodes = Mapping
+                                [(1, \<lparr>node_mark = RuleMarkNode_Blue , node_label = [Var 0], node_rooted = False\<rparr>)
+                                ,(2, \<lparr>node_mark = RuleMarkNode_None, node_label = [Var 1], node_rooted = False\<rparr>)]
+                       ,edges = Mapping [(1, \<lparr>edge_src = 2, edge_trg = 1, edge_mark = RuleMarkEdge_None, edge_label = [Var 2]\<rparr>)]\<rparr>
+           ,rule_rhs = \<lparr>nodes = Mapping 
+                                [(1, \<lparr>node_mark = RuleMarkNode_Blue , node_label = [Var 0], node_rooted = False\<rparr>)
+                                ,(2, \<lparr>node_mark = RuleMarkNode_Red, node_label = [Var 1], node_rooted = False\<rparr>)]
+                       ,edges = Mapping [(1, \<lparr>edge_src = 2, edge_trg = 1, edge_mark = RuleMarkEdge_None, edge_label = [Var 2]\<rparr>)]\<rparr>
            ,rule_interf = {1,2}\<rparr>"
 
 definition ill_blue :: ruleschema where
-"ill_blue = \<lparr>rule_ty = [''a'' \<mapsto> Lty, ''b'' \<mapsto> Lty, ''c'' \<mapsto> Lty]
-            ,rule_lhs = \<lparr>nodes = [1 \<mapsto> \<lparr>node_mark = RuleMarkNode_Blue, node_label = [Var ''a''], node_rooted = False\<rparr>
-                                 ,1 \<mapsto> \<lparr>node_mark = RuleMarkNode_Blue, node_label = [Var ''b''], node_rooted = False\<rparr>]
-                        ,edges = [1 \<mapsto> \<lparr>edge_src = 1, edge_trg = 2, edge_mark = RuleMarkEdge_None, edge_label = [Var ''c'']\<rparr>]\<rparr>
-            ,rule_rhs = \<lparr>nodes = [1 \<mapsto> \<lparr>node_mark = RuleMarkNode_Blue, node_label = [Var ''a''], node_rooted = False\<rparr>
-                                 ,1 \<mapsto> \<lparr>node_mark = RuleMarkNode_Blue, node_label = [Var ''b''], node_rooted = False\<rparr>]
-                        ,edges = [1 \<mapsto> \<lparr>edge_src = 1, edge_trg = 2, edge_mark = RuleMarkEdge_None, edge_label = [Var ''c'']\<rparr>]\<rparr>
+"ill_blue = \<lparr>rule_ty = Mapping [(0, Lty), (1, Lty), (2, Lty)]
+            ,rule_lhs = \<lparr>nodes = Mapping
+                                 [(1, \<lparr>node_mark = RuleMarkNode_Blue, node_label = [Var 0], node_rooted = False\<rparr>)
+                                 ,(2, \<lparr>node_mark = RuleMarkNode_Blue, node_label = [Var 1], node_rooted = False\<rparr>)]
+                        ,edges = Mapping [(1, \<lparr>edge_src = 1, edge_trg = 2, edge_mark = RuleMarkEdge_None, edge_label = [Var 2]\<rparr>)]\<rparr>
+            ,rule_rhs = \<lparr>nodes = Mapping
+                                 [(1, \<lparr>node_mark = RuleMarkNode_Blue, node_label = [Var 0], node_rooted = False\<rparr>)
+                                 ,(2, \<lparr>node_mark = RuleMarkNode_Blue, node_label = [Var 1], node_rooted = False\<rparr>)]
+                        ,edges = Mapping [(1, \<lparr>edge_src = 1, edge_trg = 2, edge_mark = RuleMarkEdge_None, edge_label = [Var 2]\<rparr>)]\<rparr>
             ,rule_interf = {1,2}\<rparr>"
 
 definition ill_red :: ruleschema where
-"ill_red = \<lparr>rule_ty = [''a'' \<mapsto> Lty, ''b'' \<mapsto> Lty, ''c'' \<mapsto> Lty]
-           ,rule_lhs = \<lparr>nodes = [1 \<mapsto> \<lparr>node_mark = RuleMarkNode_Red, node_label = [Var ''a''], node_rooted = False\<rparr>
-                                ,1 \<mapsto> \<lparr>node_mark = RuleMarkNode_Red, node_label = [Var ''b''], node_rooted = False\<rparr>]
-                       ,edges = [1 \<mapsto> \<lparr>edge_src = 1, edge_trg = 2, edge_mark = RuleMarkEdge_None, edge_label = [Var ''c'']\<rparr>]\<rparr>
-           ,rule_rhs = \<lparr>nodes = [1 \<mapsto> \<lparr>node_mark = RuleMarkNode_Red, node_label = [Var ''a''], node_rooted = False\<rparr>
-                                ,1 \<mapsto> \<lparr>node_mark = RuleMarkNode_Red, node_label = [Var ''b''], node_rooted = False\<rparr>]
-                       ,edges = [1 \<mapsto> \<lparr>edge_src = 1, edge_trg = 2, edge_mark = RuleMarkEdge_None, edge_label = [Var ''c'']\<rparr>]\<rparr>
+"ill_red = \<lparr>rule_ty = Mapping [(0, Lty), (1, Lty), (2, Lty)]
+           ,rule_lhs = \<lparr>nodes = Mapping
+                                [(1, \<lparr>node_mark = RuleMarkNode_Red, node_label = [Var 0], node_rooted = False\<rparr>)
+                                ,(2, \<lparr>node_mark = RuleMarkNode_Red, node_label = [Var 1], node_rooted = False\<rparr>)]
+                       ,edges = Mapping [(1, \<lparr>edge_src = 1, edge_trg = 2, edge_mark = RuleMarkEdge_None, edge_label = [Var 2]\<rparr>)]\<rparr>
+           ,rule_rhs = \<lparr>nodes = Mapping
+                                [(1, \<lparr>node_mark = RuleMarkNode_Red, node_label = [Var 0], node_rooted = False\<rparr>)
+                                ,(2, \<lparr>node_mark = RuleMarkNode_Red, node_label = [Var 1], node_rooted = False\<rparr>)]
+                       ,edges = Mapping [(1, \<lparr>edge_src = 1, edge_trg = 2, edge_mark = RuleMarkEdge_None, edge_label = [Var 2]\<rparr>)]\<rparr>
            ,rule_interf = {1,2}\<rparr>"
 
+lemma "wf_ruleschema ill_red"
+  by (simp add: ill_red_def)
+
+lemma "wf_ruleschema ill_blue"
+  by (simp add: ill_blue_def)
+
+lemma "wf_ruleschema col_red"
+  by (simp add: col_red_def)
+
+lemma "wf_ruleschema col_blue"
+  by (simp add: col_blue_def)
 
 definition twocolouring :: com where
 "twocolouring \<equiv> (RuleApp init ;; RuleSet {col_blue :: rule, col_red:: rule}!)! ;; 
@@ -73,32 +117,206 @@ definition twocolouring :: com where
 
 
 abbreviation c :: "form" where
-"c == (\<lceil>\<forall> ''x'' : Node\<rceil> \<lceil>mark \<langle>''x''\<rangle>\<rceil> \<lceil>=\<rceil> \<triangleright>\<^sub>V RuleMarkNode_None \<lceil>\<and>\<rceil> \<lceil>unrooted \<langle>''x''\<rangle>\<rceil>) \<lceil>\<and>\<rceil>
-      (\<lceil>\<forall> ''x'' : Edge\<rceil> \<lceil>mark \<langle>''x''\<rangle>\<rceil> \<lceil>=\<rceil> \<triangleright>\<^sub>E RuleMarkEdge_None)"
+"c == (\<lceil>\<forall> 0 : Node\<rceil> \<lceil>mark \<langle>0\<rangle>\<rceil> \<lceil>=\<rceil> \<triangleright>\<^sub>V RuleMarkNode_None \<lceil>\<and>\<rceil> \<lceil>unrooted \<langle>0\<rangle>\<rceil>) \<lceil>\<and>\<rceil>
+      (\<lceil>\<forall> 0 : Edge\<rceil> \<lceil>mark \<langle>0\<rangle>\<rceil> \<lceil>=\<rceil> \<triangleright>\<^sub>E RuleMarkEdge_None)"
 
 
 abbreviation d :: form where
-"d == (\<lceil>\<forall> ''x'' : Node\<rceil> \<lceil>mark \<langle>''x''\<rangle>\<rceil> \<lceil>=\<rceil> \<triangleright>\<^sub>V RuleMarkNode_Red  \<lceil>\<or>\<rceil>\<lceil>mark \<langle>''x''\<rangle>\<rceil> \<lceil>=\<rceil> \<triangleright>\<^sub>V RuleMarkNode_Blue) \<lceil>\<and>\<rceil>
-      \<lceil>\<not>\<rceil>(\<lceil>\<exists> ''x'' : Edge\<rceil> (\<lceil>src \<langle>''x''\<rangle>\<rceil> \<lceil>\<noteq>\<rceil> \<lceil>trg \<langle>''x''\<rangle>\<rceil>) \<lceil>\<and>\<rceil>
-                     \<lceil>mark \<lceil>src \<langle>''x''\<rangle>\<rceil>\<rceil> \<lceil>=\<rceil> \<lceil>mark \<lceil>trg \<langle>''x''\<rangle>\<rceil>\<rceil>)"
+"d == (\<lceil>\<forall> 0 : Node\<rceil> \<lceil>mark \<langle>0\<rangle>\<rceil> \<lceil>=\<rceil> \<triangleright>\<^sub>V RuleMarkNode_Red  \<lceil>\<or>\<rceil>\<lceil>mark \<langle>0\<rangle>\<rceil> \<lceil>=\<rceil> \<triangleright>\<^sub>V RuleMarkNode_Blue) \<lceil>\<and>\<rceil>
+      \<lceil>\<not>\<rceil>(\<lceil>\<exists> 0 : Edge\<rceil> (\<lceil>src \<langle>0\<rangle>\<rceil> \<lceil>\<noteq>\<rceil> \<lceil>trg \<langle>0\<rangle>\<rceil>) \<lceil>\<and>\<rceil>
+                     \<lceil>mark \<lceil>src \<langle>0\<rangle>\<rceil>\<rceil> \<lceil>=\<rceil> \<lceil>mark \<lceil>trg \<langle>0\<rangle>\<rceil>\<rceil>)"
 
 abbreviation e :: form where
-"e == (\<lceil>\<forall> ''x'' : Node\<rceil> (\<lceil>mark \<langle>''x''\<rangle>\<rceil> \<lceil>=\<rceil> \<triangleright>\<^sub>V RuleMarkNode_Red \<lceil>\<or>\<rceil> \<lceil>mark \<langle>''x''\<rangle>\<rceil> \<lceil>=\<rceil> \<triangleright>\<^sub>V RuleMarkNode_Blue) \<lceil>\<and>\<rceil> \<lceil>unrooted \<langle>''x''\<rangle>\<rceil>) \<lceil>\<and>\<rceil>
-      (\<lceil>\<forall> ''x'' : Edge\<rceil>  \<lceil>mark \<langle>''x''\<rangle>\<rceil> \<lceil>=\<rceil> \<triangleright>\<^sub>E RuleMarkEdge_None)"
+"e == (\<lceil>\<forall> 0 : Node\<rceil> (\<lceil>mark \<langle>0\<rangle>\<rceil> \<lceil>=\<rceil> \<triangleright>\<^sub>V RuleMarkNode_Red \<lceil>\<or>\<rceil> \<lceil>mark \<langle>0\<rangle>\<rceil> \<lceil>=\<rceil> \<triangleright>\<^sub>V RuleMarkNode_Blue) \<lceil>\<and>\<rceil> \<lceil>unrooted \<langle>0\<rangle>\<rceil>) \<lceil>\<and>\<rceil>
+      (\<lceil>\<forall> 0 : Edge\<rceil>  \<lceil>mark \<langle>0\<rangle>\<rceil> \<lceil>=\<rceil> \<triangleright>\<^sub>E RuleMarkEdge_None)"
 
 abbreviation f :: form where
-"f == (\<lceil>\<forall> ''x'' : Node\<rceil> (\<lceil>mark \<langle>''x''\<rangle>\<rceil> \<lceil>=\<rceil> \<triangleright>\<^sub>V RuleMarkNode_Red \<lceil>\<or>\<rceil> \<lceil>mark \<langle>''x''\<rangle>\<rceil> \<lceil>=\<rceil> \<triangleright>\<^sub>V RuleMarkNode_Blue \<lceil>\<or>\<rceil> 
-        \<lceil>mark \<langle>''x''\<rangle>\<rceil> \<lceil>=\<rceil> \<triangleright>\<^sub>V RuleMarkNode_None) \<lceil>\<and>\<rceil> \<lceil>unrooted \<langle>''x''\<rangle>\<rceil>) \<lceil>\<and>\<rceil>
-      (\<lceil>\<forall> ''x'' : Edge\<rceil>  \<lceil>mark \<langle>''x''\<rangle>\<rceil> \<lceil>=\<rceil> \<triangleright>\<^sub>E RuleMarkEdge_None)"
+"f == (\<lceil>\<forall> 0 : Node\<rceil> (\<lceil>mark \<langle>0\<rangle>\<rceil> \<lceil>=\<rceil> \<triangleright>\<^sub>V RuleMarkNode_Red \<lceil>\<or>\<rceil> \<lceil>mark \<langle>0\<rangle>\<rceil> \<lceil>=\<rceil> \<triangleright>\<^sub>V RuleMarkNode_Blue \<lceil>\<or>\<rceil> 
+        \<lceil>mark \<langle>0\<rangle>\<rceil> \<lceil>=\<rceil> \<triangleright>\<^sub>V RuleMarkNode_None) \<lceil>\<and>\<rceil> \<lceil>unrooted \<langle>0\<rangle>\<rceil>) \<lceil>\<and>\<rceil>
+      (\<lceil>\<forall> 0 : Edge\<rceil>  \<lceil>mark \<langle>0\<rangle>\<rceil> \<lceil>=\<rceil> \<triangleright>\<^sub>E RuleMarkEdge_None)"
 
+
+section \<open>SLP proofs\<close>
 
 lemma "eval g undefined (Slp f (init:: rule)  \<lceil>\<longleftrightarrow>\<rceil> 
-  ((\<lceil>\<exists>y: Node\<rceil> (\<lceil>\<forall>x: Node\<rceil> (\<langle>x\<rangle> \<lceil>=\<rceil> \<langle>y\<rangle> 
-    \<lceil>\<or>\<rceil> ((\<lceil>mark \<langle>x\<rangle>\<rceil> \<lceil>=\<rceil> \<triangleright>\<^sub>V RuleMarkNode_Red \<lceil>\<or>\<rceil> \<lceil>mark \<langle>x\<rangle>\<rceil> \<lceil>=\<rceil> \<triangleright>\<^sub>V RuleMarkNode_Blue \<lceil>\<or>\<rceil> \<lceil>mark \<langle>x\<rangle>\<rceil> \<lceil>=\<rceil> \<triangleright>\<^sub>V RuleMarkNode_None)\<lceil>\<and>\<rceil> \<lceil>unrooted \<langle>x\<rangle>\<rceil>)) 
-  \<lceil>\<and>\<rceil> \<lceil>mark \<langle>y\<rangle>\<rceil> \<lceil>=\<rceil> \<triangleright>\<^sub>V RuleMarkNode_Red \<lceil>\<and>\<rceil> \<lceil>unrooted \<langle>y\<rangle>\<rceil>)) \<lceil>\<and>\<rceil> (\<lceil>\<forall>x: Edge\<rceil> (\<lceil>mark \<langle>x\<rangle>\<rceil> \<lceil>=\<rceil> \<triangleright>\<^sub>E RuleMarkEdge_None))))"
-  apply (simp add: Slp_def init_def)
+  ((\<lceil>\<exists>0: Node\<rceil> (\<lceil>\<forall>1: Node\<rceil> (\<langle>1\<rangle> \<lceil>=\<rceil> \<langle>0\<rangle> 
+    \<lceil>\<or>\<rceil> ((\<lceil>mark \<langle>1\<rangle>\<rceil> \<lceil>=\<rceil> \<triangleright>\<^sub>V RuleMarkNode_Red \<lceil>\<or>\<rceil> \<lceil>mark \<langle>1\<rangle>\<rceil> \<lceil>=\<rceil> \<triangleright>\<^sub>V RuleMarkNode_Blue \<lceil>\<or>\<rceil> \<lceil>mark \<langle>1\<rangle>\<rceil> \<lceil>=\<rceil> \<triangleright>\<^sub>V RuleMarkNode_None)\<lceil>\<and>\<rceil> \<lceil>unrooted \<langle>1\<rangle>\<rceil>)) 
+  \<lceil>\<and>\<rceil> \<lceil>mark \<langle>0\<rangle>\<rceil> \<lceil>=\<rceil> \<triangleright>\<^sub>V RuleMarkNode_Red \<lceil>\<and>\<rceil> \<lceil>unrooted \<langle>0\<rangle>\<rceil>)) \<lceil>\<and>\<rceil> (\<lceil>\<forall>1: Edge\<rceil> (\<lceil>mark \<langle>1\<rangle>\<rceil> \<lceil>=\<rceil> \<triangleright>\<^sub>E RuleMarkEdge_None))))"
+  apply code_simp
+  by auto
+
+
+value "Slp f (col_blue_1::rule)"
+value "Slp f (col_blue_2::rule)"
+value "Slp f (col_red_1::rule)" 
+(* 
+lemma "eval g undefined ((Slp f (col_blue_1:: rule) \<lceil>\<or>\<rceil> Slp f (col_blue_2:: rule)) \<lceil>\<longleftrightarrow>\<rceil> 
+  (Slp f (col_red_1:: rule) \<lceil>\<or>\<rceil>  Slp f (col_red_2:: rule)))"
+  apply code_simp
   apply auto
-  sorry
+     apply (smt (z3))
+  apply (smt (z3))
+   apply (smt (z3))
+  by (smt (z3)) *)
+
+
+
+(* 
+
+lemma "eval g undefined (Slp f (col_blue:: rule) \<lceil>\<longleftrightarrow>\<rceil> Slp f (col_red:: rule))"
+   apply code_simp
+   apply auto
+  oops
+  
+
+
+  oops
+
+lemma "eval g undefined (((\<lceil>\<exists>0: Node\<rceil> (\<lceil>\<exists>1: Node\<rceil> ((\<lceil>\<forall>2: Node\<rceil> (\<langle>2\<rangle> \<lceil>=\<rceil> \<langle>0\<rangle> \<lceil>\<or>\<rceil> \<langle>2\<rangle> \<lceil>=\<rceil> \<langle>1\<rangle> \<lceil>\<or>\<rceil>
+    ((\<lceil>mark \<langle>2\<rangle>\<rceil> \<lceil>=\<rceil> \<triangleright>\<^sub>V RuleMarkNode_Red \<lceil>\<or>\<rceil> \<lceil>mark \<langle>2\<rangle>\<rceil> \<lceil>=\<rceil> \<triangleright>\<^sub>V RuleMarkNode_Blue \<lceil>\<or>\<rceil> \<lceil>mark \<langle>2\<rangle>\<rceil> \<lceil>=\<rceil> \<triangleright>\<^sub>V RuleMarkNode_None) \<lceil>\<and>\<rceil> \<lceil>unrooted \<langle>2\<rangle>\<rceil>)))
+  \<lceil>\<and>\<rceil> \<lceil>mark \<langle>0\<rangle>\<rceil> \<lceil>=\<rceil> \<triangleright>\<^sub>V RuleMarkNode_Red \<lceil>\<and>\<rceil> \<lceil>mark \<langle>1\<rangle>\<rceil> \<lceil>=\<rceil> \<triangleright>\<^sub>V RuleMarkNode_Blue \<lceil>\<and>\<rceil> \<lceil>unrooted \<langle>0\<rangle>\<rceil> \<lceil>\<and>\<rceil> \<lceil>unrooted \<langle>1\<rangle>\<rceil>
+  \<lceil>\<and>\<rceil> (\<lceil>\<exists>3: Edge\<rceil> ((\<lceil>src \<langle>3\<rangle>\<rceil> \<lceil>=\<rceil> \<langle>0\<rangle> \<lceil>\<and>\<rceil> \<lceil>trg \<langle>3\<rangle>\<rceil> \<lceil>=\<rceil> \<langle>1\<rangle>) \<lceil>\<or>\<rceil> (\<lceil>src \<langle>3\<rangle>\<rceil> \<lceil>=\<rceil> \<langle>1\<rangle> \<lceil>\<and>\<rceil> \<lceil>trg \<langle>3\<rangle>\<rceil> \<lceil>=\<rceil> \<langle>0\<rangle>)) )))) \<lceil>\<and>\<rceil> (\<lceil>\<forall>4:Edge\<rceil> (\<lceil>mark \<langle>4\<rangle>\<rceil> \<lceil>=\<rceil> \<triangleright>\<^sub>E RuleMarkEdge_None)))  \<lceil>\<longrightarrow>\<rceil>  Slp f (col_blue:: rule))"
+  apply code_simp
+  apply auto
+   apply (erule notE)
+   apply (smt (z3) conv_mark_node.elims mark_eq_node.simps(12) mark_eq_node.simps(15) mark_eq_node.simps(23) mark_eq_node.simps(24) mark_eq_node.simps(26) rulemark_node.distinct(13))
+  apply (erule notE)
+  apply (rule spec)
+  oops  
+
+
+  text \<open>
+    Slp f col_blue implies rule
+  \<close>
+*)
+lemma x[simp]:"mark_eq_node (conv_mark_node HostMarkNode_Red) RuleMarkNode_Red"
+  by simp
+
+
+lemma xxx: "\<And>e. \<forall>e\<in>Mapping.keys (edges g).
+            (\<exists>y. Mapping.lookup (nodes g) (edge_trg (the (Mapping.lookup (edges g) e))) = Some y) \<and>
+            (\<exists>y. Mapping.lookup (nodes g) (edge_src (the (Mapping.lookup (edges g) e))) = Some y) \<Longrightarrow>
+         edge_src (the (Mapping.lookup (edges g) e)) \<in> Mapping.keys (nodes g) \<Longrightarrow>
+         edge_trg (the (Mapping.lookup (edges g) e)) \<in> Mapping.keys (nodes g) \<Longrightarrow>
+         \<forall>e\<in>Mapping.keys (edges g). mark_eq_edge (conv_mark_edge (edge_mark (the (Mapping.lookup (edges g) e)))) RuleMarkEdge_None \<Longrightarrow>
+         \<forall>n\<in>Mapping.keys (nodes g).
+            mark_eq_node (conv_mark_node (node_mark (the (Mapping.lookup (nodes g) n)))) RuleMarkNode_Blue \<longrightarrow>
+            (\<forall>na\<in>Mapping.keys (nodes g).
+                mark_eq_node (conv_mark_node (node_mark (the (Mapping.lookup (nodes g) na)))) RuleMarkNode_Red \<longrightarrow>
+                n = na \<or>
+                na = n \<or>
+                (\<exists>nb\<in>Mapping.keys (nodes g).
+                    nb \<noteq> na \<and>
+                    nb \<noteq> n \<and>
+                    (\<not> mark_eq_node (conv_mark_node (node_mark (the (Mapping.lookup (nodes g) nb)))) RuleMarkNode_Red \<and>
+                     \<not> mark_eq_node (conv_mark_node (node_mark (the (Mapping.lookup (nodes g) nb)))) RuleMarkNode_Blue \<and>
+                     \<not> mark_eq_node (conv_mark_node (node_mark (the (Mapping.lookup (nodes g) nb)))) RuleMarkNode_None \<or>
+                     node_rooted (the (Mapping.lookup (nodes g) nb)))) \<or>
+                node_rooted (the (Mapping.lookup (nodes g) na)) \<or>
+                node_rooted (the (Mapping.lookup (nodes g) n)) \<or>
+                (\<forall>e\<in>Mapping.keys (edges g). edge_src (the (Mapping.lookup (edges g) e)) = n \<longrightarrow> edge_trg (the (Mapping.lookup (edges g) e)) \<noteq> na)) \<Longrightarrow>
+         \<forall>n\<in>Mapping.keys (nodes g).
+            \<forall>na\<in>Mapping.keys (nodes g).
+               mark_eq_node (conv_mark_node (node_mark (the (Mapping.lookup (nodes g) na)))) RuleMarkNode_Blue \<longrightarrow>
+               mark_eq_node (conv_mark_node (node_mark (the (Mapping.lookup (nodes g) n)))) RuleMarkNode_Red \<longrightarrow>
+               n = na \<or>
+               na = n \<or>
+               (\<exists>nb\<in>Mapping.keys (nodes g).
+                   nb \<noteq> n \<and>
+                   nb \<noteq> na \<and>
+                   (\<not> mark_eq_node (conv_mark_node (node_mark (the (Mapping.lookup (nodes g) nb)))) RuleMarkNode_Red \<and>
+                    \<not> mark_eq_node (conv_mark_node (node_mark (the (Mapping.lookup (nodes g) nb)))) RuleMarkNode_Blue \<and>
+                    \<not> mark_eq_node (conv_mark_node (node_mark (the (Mapping.lookup (nodes g) nb)))) RuleMarkNode_None \<or>
+                    node_rooted (the (Mapping.lookup (nodes g) nb)))) \<or>
+               node_rooted (the (Mapping.lookup (nodes g) n)) \<or>
+               node_rooted (the (Mapping.lookup (nodes g) na)) \<or>
+               (\<forall>e\<in>Mapping.keys (edges g). edge_src (the (Mapping.lookup (edges g) e)) = n \<longrightarrow> edge_trg (the (Mapping.lookup (edges g) e)) \<noteq> na) \<Longrightarrow>
+         mark_eq_node (conv_mark_node (node_mark (the (Mapping.lookup (nodes g) (edge_trg (the (Mapping.lookup (edges g) e))))))) RuleMarkNode_Blue \<Longrightarrow>
+         mark_eq_node (conv_mark_node (node_mark (the (Mapping.lookup (nodes g) (edge_src (the (Mapping.lookup (edges g) e))))))) RuleMarkNode_Red \<Longrightarrow>
+         \<forall>n\<in>Mapping.keys (nodes g).
+            n = edge_src (the (Mapping.lookup (edges g) e)) \<or>
+            n = edge_trg (the (Mapping.lookup (edges g) e)) \<or>
+            (mark_eq_node (conv_mark_node (node_mark (the (Mapping.lookup (nodes g) n)))) RuleMarkNode_Red \<or>
+             mark_eq_node (conv_mark_node (node_mark (the (Mapping.lookup (nodes g) n)))) RuleMarkNode_Blue \<or>
+             mark_eq_node (conv_mark_node (node_mark (the (Mapping.lookup (nodes g) n)))) RuleMarkNode_None) \<and>
+            \<not> node_rooted (the (Mapping.lookup (nodes g) n)) \<Longrightarrow>
+         \<not> node_rooted (the (Mapping.lookup (nodes g) (edge_src (the (Mapping.lookup (edges g) e))))) \<Longrightarrow>
+         \<not> node_rooted (the (Mapping.lookup (nodes g) (edge_trg (the (Mapping.lookup (edges g) e))))) \<Longrightarrow> e \<in> Mapping.keys (edges g) \<Longrightarrow> False"
+proof -
+  fix e :: nat
+  assume a1: "mark_eq_node (conv_mark_node (node_mark (the (Mapping.lookup (nodes g) (edge_trg (the (Mapping.lookup (edges g) e))))))) RuleMarkNode_Blue"
+  assume a2: "mark_eq_node (conv_mark_node (node_mark (the (Mapping.lookup (nodes g) (edge_src (the (Mapping.lookup (edges g) e))))))) RuleMarkNode_Red"
+  assume a3: "edge_trg (the (Mapping.lookup (edges g) e)) \<in> Mapping.keys (nodes g)"
+  assume a4: "\<not> node_rooted (the (Mapping.lookup (nodes g) (edge_src (the (Mapping.lookup (edges g) e)))))"
+  assume a5: "\<not> node_rooted (the (Mapping.lookup (nodes g) (edge_trg (the (Mapping.lookup (edges g) e)))))"
+  assume a6: "edge_src (the (Mapping.lookup (edges g) e)) \<in> Mapping.keys (nodes g)"
+  assume a7: "\<forall>n\<in>Mapping.keys (nodes g). \<forall>na\<in>Mapping.keys (nodes g). mark_eq_node (conv_mark_node (node_mark (the (Mapping.lookup (nodes g) na)))) RuleMarkNode_Blue \<longrightarrow> mark_eq_node (conv_mark_node (node_mark (the (Mapping.lookup (nodes g) n)))) RuleMarkNode_Red \<longrightarrow> n = na \<or> na = n \<or> (\<exists>nb\<in>Mapping.keys (nodes g). nb \<noteq> n \<and> nb \<noteq> na \<and> (\<not> mark_eq_node (conv_mark_node (node_mark (the (Mapping.lookup (nodes g) nb)))) RuleMarkNode_Red \<and> \<not> mark_eq_node (conv_mark_node (node_mark (the (Mapping.lookup (nodes g) nb)))) RuleMarkNode_Blue \<and> \<not> mark_eq_node (conv_mark_node (node_mark (the (Mapping.lookup (nodes g) nb)))) RuleMarkNode_None \<or> node_rooted (the (Mapping.lookup (nodes g) nb)))) \<or> node_rooted (the (Mapping.lookup (nodes g) n)) \<or> node_rooted (the (Mapping.lookup (nodes g) na)) \<or> (\<forall>e\<in>Mapping.keys (edges g). edge_src (the (Mapping.lookup (edges g) e)) = n \<longrightarrow> edge_trg (the (Mapping.lookup (edges g) e)) \<noteq> na)"
+  assume a8: "\<forall>n\<in>Mapping.keys (nodes g). n = edge_src (the (Mapping.lookup (edges g) e)) \<or> n = edge_trg (the (Mapping.lookup (edges g) e)) \<or> (mark_eq_node (conv_mark_node (node_mark (the (Mapping.lookup (nodes g) n)))) RuleMarkNode_Red \<or> mark_eq_node (conv_mark_node (node_mark (the (Mapping.lookup (nodes g) n)))) RuleMarkNode_Blue \<or> mark_eq_node (conv_mark_node (node_mark (the (Mapping.lookup (nodes g) n)))) RuleMarkNode_None) \<and> \<not> node_rooted (the (Mapping.lookup (nodes g) n))"
+  assume a9: "e \<in> Mapping.keys (edges g)"
+  obtain nn :: "nat \<Rightarrow> nat \<Rightarrow> nat" where
+"\<forall>x0 x1. (\<exists>v2. v2 \<in> Mapping.keys (nodes g) \<and> v2 \<noteq> x1 \<and> v2 \<noteq> x0 \<and> (\<not> mark_eq_node (conv_mark_node (node_mark (the (Mapping.lookup (nodes g) v2)))) RuleMarkNode_Red \<and> \<not> mark_eq_node (conv_mark_node (node_mark (the (Mapping.lookup (nodes g) v2)))) RuleMarkNode_Blue \<and> \<not> mark_eq_node (conv_mark_node (node_mark (the (Mapping.lookup (nodes g) v2)))) RuleMarkNode_None \<or> node_rooted (the (Mapping.lookup (nodes g) v2)))) = (nn x0 x1 \<in> Mapping.keys (nodes g) \<and> nn x0 x1 \<noteq> x1 \<and> nn x0 x1 \<noteq> x0 \<and> (\<not> mark_eq_node (conv_mark_node (node_mark (the (Mapping.lookup (nodes g) (nn x0 x1))))) RuleMarkNode_Red \<and> \<not> mark_eq_node (conv_mark_node (node_mark (the (Mapping.lookup (nodes g) (nn x0 x1))))) RuleMarkNode_Blue \<and> \<not> mark_eq_node (conv_mark_node (node_mark (the (Mapping.lookup (nodes g) (nn x0 x1))))) RuleMarkNode_None \<or> node_rooted (the (Mapping.lookup (nodes g) (nn x0 x1)))))"
+    by moura
+  then have f10: "\<forall>n. n \<notin> Mapping.keys (nodes g) \<or> (\<forall>na. (na \<notin> Mapping.keys (nodes g) \<or> \<not> mark_eq_node (conv_mark_node (node_mark (the (Mapping.lookup (nodes g) na)))) RuleMarkNode_Blue \<or> \<not> mark_eq_node (conv_mark_node (node_mark (the (Mapping.lookup (nodes g) n)))) RuleMarkNode_Red) \<or> n = na \<or> na = n \<or> nn na n \<in> Mapping.keys (nodes g) \<and> nn na n \<noteq> n \<and> nn na n \<noteq> na \<and> (\<not> mark_eq_node (conv_mark_node (node_mark (the (Mapping.lookup (nodes g) (nn na n))))) RuleMarkNode_Red \<and> \<not> mark_eq_node (conv_mark_node (node_mark (the (Mapping.lookup (nodes g) (nn na n))))) RuleMarkNode_Blue \<and> \<not> mark_eq_node (conv_mark_node (node_mark (the (Mapping.lookup (nodes g) (nn na n))))) RuleMarkNode_None \<or> node_rooted (the (Mapping.lookup (nodes g) (nn na n)))) \<or> node_rooted (the (Mapping.lookup (nodes g) n)) \<or> node_rooted (the (Mapping.lookup (nodes g) na)) \<or> (\<forall>nb. (nb \<notin> Mapping.keys (edges g) \<or> edge_src (the (Mapping.lookup (edges g) nb)) \<noteq> n) \<or> edge_trg (the (Mapping.lookup (edges g) nb)) \<noteq> na))"
+    using a7 by (simp add: Ball_def_raw Bex_def_raw)
+  have "conv_mark_node (node_mark (the (Mapping.lookup (nodes g) (edge_trg (the (Mapping.lookup (edges g) e)))))) \<noteq> RuleMarkNode_Green"
+    using a1 by force
+  then show False
+    using f10 a9 a8 a6 a5 a4 a3 a2 a1 by (smt (z3) conv_mark_node.elims mark_eq_node.simps(12) mark_eq_node.simps(15) mark_eq_node.simps(16) mark_eq_node.simps(23) rulemark_node.distinct(13))
+qed
+
+lemma "\<lbrakk>wf_ruleschema col_blue_1; wf_ruleschema col_blue_2; wf_graph g\<rbrakk> 
+  \<Longrightarrow> eval g undefined ((Slp f (col_blue_1:: rule) \<lceil>\<or>\<rceil> Slp f (col_blue_2:: rule))  \<lceil>\<longleftrightarrow>\<rceil>   
+  (\<lceil>\<exists>0: Node\<rceil> (\<lceil>\<exists>1: Node\<rceil> ((\<lceil>\<forall>2: Node\<rceil> (\<langle>2\<rangle> \<lceil>=\<rceil> \<langle>0\<rangle> \<lceil>\<or>\<rceil> \<langle>2\<rangle> \<lceil>=\<rceil> \<langle>1\<rangle> \<lceil>\<or>\<rceil>
+    ((\<lceil>mark \<langle>2\<rangle>\<rceil> \<lceil>=\<rceil> \<triangleright>\<^sub>V RuleMarkNode_Red \<lceil>\<or>\<rceil> \<lceil>mark \<langle>2\<rangle>\<rceil> \<lceil>=\<rceil> \<triangleright>\<^sub>V RuleMarkNode_Blue \<lceil>\<or>\<rceil> \<lceil>mark \<langle>2\<rangle>\<rceil> \<lceil>=\<rceil> \<triangleright>\<^sub>V RuleMarkNode_None) \<lceil>\<and>\<rceil> \<lceil>unrooted \<langle>2\<rangle>\<rceil>)))
+  \<lceil>\<and>\<rceil> \<lceil>mark \<langle>0\<rangle>\<rceil> \<lceil>=\<rceil> \<triangleright>\<^sub>V RuleMarkNode_Red \<lceil>\<and>\<rceil> \<lceil>mark \<langle>1\<rangle>\<rceil> \<lceil>=\<rceil> \<triangleright>\<^sub>V RuleMarkNode_Blue \<lceil>\<and>\<rceil> \<lceil>unrooted \<langle>0\<rangle>\<rceil> \<lceil>\<and>\<rceil> \<lceil>unrooted \<langle>1\<rangle>\<rceil>
+  \<lceil>\<and>\<rceil> (\<lceil>\<exists>3: Edge\<rceil> ((\<lceil>src \<langle>3\<rangle>\<rceil> \<lceil>=\<rceil> \<langle>0\<rangle> \<lceil>\<and>\<rceil> \<lceil>trg \<langle>3\<rangle>\<rceil> \<lceil>=\<rceil> \<langle>1\<rangle>) \<lceil>\<or>\<rceil> (\<lceil>src \<langle>3\<rangle>\<rceil> \<lceil>=\<rceil> \<langle>1\<rangle> \<lceil>\<and>\<rceil> \<lceil>trg \<langle>3\<rangle>\<rceil> \<lceil>=\<rceil> \<langle>0\<rangle>)) )))) \<lceil>\<and>\<rceil> (\<lceil>\<forall>4:Edge\<rceil> (\<lceil>mark \<langle>4\<rangle>\<rceil> \<lceil>=\<rceil> \<triangleright>\<^sub>E RuleMarkEdge_None)))"
+  apply code_simp
+  apply safe
+  apply auto
+     apply (metis (no_types, lifting))
+    apply (metis (no_types, hide_lams))
+   apply (rule xxx)
+              apply blast+
+  apply (rule xxx)
+             apply blast+
+  by (metis (no_types, hide_lams))+
+
+
+
+  
+  
+  
+(*
+lemma "eval g undefined (Slp f (col_red:: rule)  \<lceil>\<longrightarrow>\<rceil>  
+  (\<lceil>\<exists>0: Node\<rceil> (\<lceil>\<exists>1: Node\<rceil> ((\<lceil>\<forall>2: Node\<rceil> (\<langle>2\<rangle> \<lceil>=\<rceil> \<langle>0\<rangle> \<lceil>\<or>\<rceil> \<langle>2\<rangle> \<lceil>=\<rceil> \<langle>1\<rangle> \<lceil>\<or>\<rceil>
+    ((\<lceil>mark \<langle>2\<rangle>\<rceil> \<lceil>=\<rceil> \<triangleright>\<^sub>V RuleMarkNode_Red \<lceil>\<or>\<rceil> \<lceil>mark \<langle>2\<rangle>\<rceil> \<lceil>=\<rceil> \<triangleright>\<^sub>V RuleMarkNode_Blue \<lceil>\<or>\<rceil> \<lceil>mark \<langle>2\<rangle>\<rceil> \<lceil>=\<rceil> \<triangleright>\<^sub>V RuleMarkNode_None) \<lceil>\<and>\<rceil> \<lceil>unrooted \<langle>2\<rangle>\<rceil>)))
+  \<lceil>\<and>\<rceil> \<lceil>mark \<langle>0\<rangle>\<rceil> \<lceil>=\<rceil> \<triangleright>\<^sub>V RuleMarkNode_Red \<lceil>\<and>\<rceil> \<lceil>mark \<langle>1\<rangle>\<rceil> \<lceil>=\<rceil> \<triangleright>\<^sub>V RuleMarkNode_Blue \<lceil>\<and>\<rceil> \<lceil>unrooted \<langle>0\<rangle>\<rceil> \<lceil>\<and>\<rceil> \<lceil>unrooted \<langle>1\<rangle>\<rceil>
+  \<lceil>\<and>\<rceil> (\<lceil>\<exists>3: Edge\<rceil> ((\<lceil>src \<langle>3\<rangle>\<rceil> \<lceil>=\<rceil> \<langle>0\<rangle> \<lceil>\<and>\<rceil> \<lceil>trg \<langle>3\<rangle>\<rceil> \<lceil>=\<rceil> \<langle>1\<rangle>) \<lceil>\<or>\<rceil> (\<lceil>src \<langle>3\<rangle>\<rceil> \<lceil>=\<rceil> \<langle>1\<rangle> \<lceil>\<and>\<rceil> \<lceil>trg \<langle>3\<rangle>\<rceil> \<lceil>=\<rceil> \<langle>0\<rangle>)) )))) \<lceil>\<and>\<rceil> (\<lceil>\<forall>4:Edge\<rceil> (\<lceil>mark \<langle>4\<rangle>\<rceil> \<lceil>=\<rceil> \<triangleright>\<^sub>E RuleMarkEdge_None)))"
+  apply code_simp
+  by auto  
+
+lemma "eval g undefined (Slp f (col_red:: rule)  \<lceil>\<longleftrightarrow>\<rceil>
+  ((\<lceil>\<exists>0: Node\<rceil> 
+    (\<lceil>\<exists>1: Node\<rceil> 
+      ((\<lceil>\<forall>2: Node\<rceil> (\<langle>2\<rangle> \<lceil>=\<rceil> \<langle>0\<rangle> \<lceil>\<or>\<rceil> \<langle>2\<rangle> \<lceil>=\<rceil> \<langle>1\<rangle> \<lceil>\<or>\<rceil>
+        ((\<lceil>mark \<langle>2\<rangle>\<rceil> \<lceil>=\<rceil> \<triangleright>\<^sub>V RuleMarkNode_Red \<lceil>\<or>\<rceil> \<lceil>mark \<langle>2\<rangle>\<rceil> \<lceil>=\<rceil> \<triangleright>\<^sub>V RuleMarkNode_Blue \<lceil>\<or>\<rceil> \<lceil>mark \<langle>2\<rangle>\<rceil> \<lceil>=\<rceil> \<triangleright>\<^sub>V RuleMarkNode_None) \<lceil>\<and>\<rceil> \<lceil>unrooted \<langle>2\<rangle>\<rceil>) ))
+  \<lceil>\<and>\<rceil> \<lceil>mark \<langle>0\<rangle>\<rceil> \<lceil>=\<rceil> \<triangleright>\<^sub>V RuleMarkNode_Red \<lceil>\<and>\<rceil> \<lceil>mark \<langle>1\<rangle>\<rceil> \<lceil>=\<rceil> \<triangleright>\<^sub>V RuleMarkNode_Blue \<lceil>\<and>\<rceil> \<lceil>unrooted \<langle>0\<rangle>\<rceil> \<lceil>\<and>\<rceil> \<lceil>unrooted \<langle>1\<rangle>\<rceil>
+  \<lceil>\<and>\<rceil> (\<lceil>\<exists>3: Edge\<rceil> ((\<lceil>src \<langle>3\<rangle>\<rceil> \<lceil>=\<rceil> \<langle>0\<rangle> \<lceil>\<and>\<rceil> \<lceil>trg \<langle>3\<rangle>\<rceil> \<lceil>=\<rceil> \<langle>1\<rangle>) \<lceil>\<or>\<rceil> (\<lceil>src \<langle>3\<rangle>\<rceil> \<lceil>=\<rceil> \<langle>1\<rangle> \<lceil>\<and>\<rceil> \<lceil>trg \<langle>3\<rangle>\<rceil> \<lceil>=\<rceil> \<langle>0\<rangle>)) )))) \<lceil>\<and>\<rceil> (\<lceil>\<forall>4:Edge\<rceil> (\<lceil>mark \<langle>4\<rangle>\<rceil> \<lceil>=\<rceil> \<triangleright>\<^sub>E RuleMarkEdge_None))))"
+  apply code_simp
+  apply auto
+  oops
+ *)
+  
+  
+lemma "eval g undefined (Slp f (unmark :: rule)  \<lceil>\<longleftrightarrow>\<rceil>  
+  (\<lceil>\<exists>1: Node\<rceil> ((\<lceil>\<forall>0: Node\<rceil> (\<langle>0\<rangle> \<lceil>=\<rceil> \<langle>1\<rangle> \<lceil>\<or>\<rceil> 
+    ((\<lceil>mark \<langle>0\<rangle>\<rceil> \<lceil>=\<rceil> \<triangleright>\<^sub>V RuleMarkNode_Red \<lceil>\<or>\<rceil> \<lceil>mark \<langle>0\<rangle>\<rceil> \<lceil>=\<rceil> \<triangleright>\<^sub>V RuleMarkNode_Blue \<lceil>\<or>\<rceil> \<lceil>mark \<langle>0\<rangle>\<rceil> \<lceil>=\<rceil> \<triangleright>\<^sub>V RuleMarkNode_None) \<lceil>\<and>\<rceil> \<lceil>unrooted \<langle>0\<rangle>\<rceil>)))
+  \<lceil>\<and>\<rceil> \<lceil>mark \<langle>1\<rangle>\<rceil> \<lceil>=\<rceil>\<triangleright>\<^sub>V RuleMarkNode_None \<lceil>\<and>\<rceil> \<lceil>unrooted \<langle>1\<rangle>\<rceil>)) \<lceil>\<and>\<rceil> (\<lceil>\<forall>4:Edge\<rceil> (\<lceil>mark \<langle>4\<rangle>\<rceil> \<lceil>=\<rceil> \<triangleright>\<^sub>E RuleMarkEdge_None)))"
+  apply code_simp
+  by auto
+
+
+
 
 
 lemma c_impl_f : "eval g undefined (c \<lceil>\<longrightarrow>\<rceil> f)" 
