Common.thy
@@ -1,12 +1,16 @@
 theory Common
-  imports Main
+  imports Main "HOL-Library.Mapping"
 begin
 
+fun mfold :: "('k :: linorder, 'v) mapping \<Rightarrow> ('k \<times> 'v \<Rightarrow> 'c \<Rightarrow> 'c) \<Rightarrow> 'c \<Rightarrow> 'c" where
+"mfold m r i = 
+  (let f = \<lambda>k a. r (k, the (Mapping.lookup m k)) a in foldr f (Mapping.ordered_keys m) i)"
+(* 
 fun mfold :: "('a :: linorder \<rightharpoonup> 'b) \<Rightarrow> ('a \<times> 'b \<Rightarrow> 'c \<Rightarrow> 'c) \<Rightarrow> 'c \<Rightarrow> 'c" where
 "mfold m f i = (let v = sorted_list_of_set (dom m);
                     z = zip v (map (the \<circ> m) v)
                 in fold f z i)"
-
+ *)
 (* https://stackoverflow.com/questions/28633353/converting-a-set-to-a-list-in-isabelle *)
 definition set_to_list :: "'a set \<Rightarrow> 'a list"
   where "set_to_list s = (SOME l. set l = s)"
